\documentclass[class=article, crop=false]{standalone}
\input{../../Preamble}

\fancyhf{}
\lhead{Kyle Chui}
\rhead{Page \thepage}
\pagestyle{fancy}

\begin{document}
  \section{Lecture 17}
  \subsection{Multiple Point Formulas for Numerical Differentiation}
  We have the $n + 1$ points $(x_0, f(x_0)),\dotsc,(x_n, f(x_n))$. We have that $f(x) = \text{Lagrange Interpolation} + \text{Error}$, so
  \[
    f(x) = \sum_{k=0}^{n}f(x_k)\ell_k(x) + \frac{(x - x_0)\dotsb(x - x_n)}{(n + 1)!}f^{(n + 1)}(\xi_x).\tag*{$\xi_x\in (x_0, x_n)$}
  \]
  We then approximate $f'(x)$ by
  \[
    f'(x) = \sum_{k=0}^{n} f(x_k)\ell_k'(x) + D_x\paren{\frac{(x - x_0)\dotsb(x - x_n)}{(n + 1)!}}f^{(n + 1)}(\xi_x) + D_x(f^{(n + 1)}(\xi_x))\cdot \frac{(x - x_0)\dotsb(x - x_n)}{(n + 1)!}.
  \]
  If we only consider the derivative at our interpolation points, i.e. $x_j$, then we have
  \[
    f'(x_j) = \sum_{k=0}^{n} f(x_k)\ell_k'(x_j) + \frac{(x_j - x_0)\dotsb(x_j - x_{j - 1})(x_j - x_{j + 1})\dotsb(x_j - x_n)}{(n + 1)!}f^{(n + 1)}(\xi_x).
  \]
  We call the above the $n + 1$ point formula.
  \begin{note}{}
    More points yield more accurate approximations, but also increase the number of operations which leads to round-off error. Because of this, too many points can also be a bad thing, and two, three, and five point formulas are the most common.
  \end{note}
  \subsection{Three Point Formula}
  \subsubsection{Three Point Formula (Left)}
  Suppose we are given the three points $(x_0, f(x_0)), (x_1, f(x_1)), (x_2, f(x_2))$, where $x_0, x_1, x_2$ are equidistant points. Then we have
  \begin{align*}
    \ell_0(x) &= \frac{(x - x_1)(x - x_2)}{(x_0 - x_1)(x_0 - x_2)}, \\
    \ell_1(x) &= \frac{(x - x_0)(x - x_2)}{(x_1 - x_0)(x_1 - x_2)}, \\
    \ell_2(x) &= \frac{(x - x_0)(x - x_1)}{(x_2 - x_0)(x_2 - x_1)}.
  \end{align*}
  Hence their derivatives are
  \begin{align*}
    \ell_0'(x) &= \frac{x - x_2 + x - x_1}{(x_0 - x_1)(x_0 - x_2)}, \\
    \ell_1'(x) &= \frac{x - x_2 + x - x_0}{(x_1 - x_0)(x_1 - x_2)}, \\
    \ell_2'(x) &= \frac{x - x_1 + x - x_0}{(x_2 - x_1)(x_2 - x_0)}.
  \end{align*}
  Therefore
  \[
    f'(x_j) = \frac{2x_j - x_2 - x_1}{2h^2}f(x_0) + \frac{2x_j - x_2 - x_0}{-h^2}f(x_1) + \frac{2x_j - x_1 - x_0}{2h^2}f(x_2) + \prod_{\substack{k = 0\\k\neq j}}^{2} \frac{x_j - x_k}{(n + 1)!}\cdot f^{(3)}(\xi_{x_j}).
  \]
  If we take $x^* = x_0$, with $x_1 = x^* + h$ and $x_2 = x^* + 2h$, we can simplify to get
  \[
    f'(x^*) = \frac{1}{2h}\paren{-3f(x^*) + 4f(x^* + h) - f(x^* + 2h)} - \frac{1}{3}h^2f^{(3)}(\xi_x).
  \]
  \subsubsection{Three Point Formula (Central)}
  \[
    f'(x^*) = \frac{f(x^* + h) - f(x^* - h)}{2h} - \frac{h^2}{6}f^{(3)}(\xi_*).
  \]
  \subsubsection{Three Point Formula (Right)}
  \[
    f'(x^*) = \frac{1}{2h}\paren{3f(x^*) - 4f(x^* - h) + f(x^* - 2h)} + \frac{1}{3}h^2f^{(3)}(\xi_x).
  \]
  \subsection{Five Point Formula}
  \subsubsection{Five Point Formula (Left)}
  \[
    f'(x) = \frac{1}{12h}\paren{-25f(x^*) + 48f(x^* + h) - 36f(x^* + 2h) + 16f(x^* + 3h) - 3f(x^* + 4h)} + \frac{h^4}{5}f^{(5)}(\xi_*).
  \]
  \subsubsection{Five Point Formula (Central)}
  \[
    f'(x) = \frac{1}{12h}\paren{f(x^* - 2h) - 8f(x^* - h) + 8f(x^* + h) - f(x^* + 2h)} + \frac{h^4}{30}f^{(5)}(\xi_*).
  \]
\end{document}
