\documentclass[class=article, crop=false]{standalone}
\input{../../Preamble}

\fancyhf{}
\lhead{Kyle Chui}
\rhead{Page \thepage}
\pagestyle{fancy}

\begin{document}
  \section{Lecture 6}
  \begin{theorem}{The Law of Total Probability}
    Let $A\sse \Omega$ be an event and $B_1,B_2\dotsc,B_n\sse \Omega$ be mutually exclusive events so that $\P[B_j]\neq 0$ and
    \[
      A\sse \bigcup_{j = 1}^n B_j.
    \]
    Then
    \[
      \P[A] = \sum_{j=1}^{n}\P[A\mid B_j]\P[B_j].
    \]
    \begin{proof}
      As $A\sse \bigcup_{j = 1}^n B_j$ we have
      \[
        A = A\cap \left[\bigcup_{j = 1}^n B_j\right] = \bigcup_{j = 1}^n (A\cap B_j).
      \]
      As all of the $B_j$ are mutually exclusive, so are $A\cap B_j$. Hence
      \begin{align*}
        \P[A] &= \P\left[\bigcup_{j = 1}^n (A\cap B_j)\right] \\
              &= \sum_{j=1}^{n}\P[A\cap B_j] \\
              &= \sum_{j=1}^{n}\P[A\mid B_j]\P[B_j].
      \end{align*}
    \end{proof}
  \end{theorem}
  \begin{note}{}
    The same result is true if we have a countable number of events $B_1, B_2,\dotsc$.
  \end{note}
  \subsection{Bayes' Theorem}
  \begin{theorem}{Bayes' Theorem}
    If $A, B\sse \Omega$ are events so that $\P[A], \P[B]\neq 0$ then
    \[
      \P[B\mid A] = \frac{\P[A\mid B]\P[B]}{\P[A]}
    \]
    \begin{proof}
      By definition, we have
      \begin{align*}
        \P[B\mid A] &= \frac{\P[A\cap B]}{\P[A]} \\
                    &= \frac{\P[A\mid B]\P[B]}{\P[A]}.
      \end{align*}
    \end{proof}
  \end{theorem}
  \begin{theorem}{Bayes' Theorem (Improved Version)}
    If $A\sse \Omega$ is an event and $B_1, B_2,\dotsc, B_n\sse \Omega$ are mutually exclusive events so that $\P[A], \P[B_j]\neq 0$ and
    \[
      A\sse \bigcup_{j = 1}^nB_j,
    \]
    then for any $1\leq k\leq n$ we have
    \[
      \P[B_k\mid A] = \frac{\P[A\mid B_k]\P[B_k]}{\sum_{j=1}^{n}\P[A\mid B_j]\P[B_j]}.
    \]
    \begin{proof}
      The Law of Total Probability tells us that
      \[
        \P[A] = \sum_{j=1}^{n}\P[A\mid B_j]\P[B_j].
      \]
      Hence by Bayes' Theorem we have
      \begin{align*}
        \P[B_k\mid A] &= \frac{\P[A\mid B_k]\P[B_k]}{\P[A]} \\
                      &= \frac{\P[A\mid B_k]\P[B_k]}{\sum_{j=1}^{n}\P[A\mid B_j]\P[B_j]}.
      \end{align*}
    \end{proof}
  \end{theorem}
\end{document}
